WIP: Revamp handling of pure returns in framing tactic

ulib/experimental/Steel.Effect.Common.fsti
@@ -4,11 +4,12 @@ open Steel.Memory
 module Sem = Steel.Semantics.Hoare.MST
 open Steel.Semantics.Instantiate
 
-
 irreducible let framing_implicit : unit = ()
 
 let delay (p:Type0) : Type0 = p
 let annot_sub_post (p:Type0) : Type0 = p
+let return_pre (p:slprop u#1) : slprop u#1 = p
+let return_post (#a:Type) (p:a -> slprop u#1) : a -> slprop u#1 = p
 
 type pre_t = slprop u#1
 type post_t (a:Type) = a -> slprop u#1
@@ -77,6 +78,24 @@ val lemma_sl_implies_refl (p:slprop) : Lemma
   (ensures p `sl_implies` p)
 
 open FStar.Tactics
+
+(* TODO: Remove once it lands in master ulib/ *)
+exception Yes
+
+let name_appears_in (nm:name) (t:term) : Tac bool =
+  let ff (t : term) : Tac term =
+    match t with
+    | Tv_FVar fv ->
+      if inspect_fv fv = nm then
+        raise Yes;
+      t
+    | t -> t
+  in
+  try ignore (visit_tm ff t); false with
+  | Yes -> true
+  | e -> raise e
+
+let term_appears_in (t:term) (i:term) : Tac bool = name_appears_in (explode_qn (term_to_string t)) i
 
 let atom : eqtype = int
 
@@ -615,6 +634,23 @@ let identity_left (#a:Type) (eq:equiv a) (m:cm a eq) (x:a)
   = CM?.identity m x;
     EQ?.symmetry eq (CM?.mult m (CM?.unit m) x) x
 
+let identity_right (#a:Type) (eq:equiv a) (m:cm a eq) (x:a)
+  : Lemma (EQ?.eq eq (CM?.mult m x (CM?.unit m)) x)
+  = admit()
+
+let identity_right_diff (#a:Type) (eq:equiv a) (m:cm a eq) (x y:a) : Lemma
+  (requires EQ?.eq eq x y)
+  (ensures EQ?.eq eq (CM?.mult m x (CM?.unit m)) y)
+  = admit()
+
+let rec n_identity_left (n:int) (eq m:term) : Tac unit
+  = if n = 0 then apply_lemma (`(EQ?.reflexivity (`#eq)))
+    else (
+      apply_lemma (`identity_right_diff (`#eq) (`#m));
+      later();
+      n_identity_left (n-1) eq m
+    )
+
 let equivalent_sorted (#a:Type) (eq:equiv a) (m:cm a eq) (am:amap a) (l1 l2 l1' l2':list atom)
     : Lemma (requires
               sort l1 == sort l1' /\
@@ -795,6 +831,100 @@ let canon_monoid (eq:term) (m:term) : Tac unit =
 let canon' () : Tac unit =
   canon_monoid (`Steel.Memory.Tactics.req) (`Steel.Memory.Tactics.rm)
 
+(* A Variant of canon to collect all slprops in the context into the return_post term,
+   and set all extra uvars to emp *)
+
+/// Puts the term containing return_post at the top.
+/// Returns the atom corresponding to return_post, and the list with the atom removed
+let rec return_at_top (l:list atom) (am:amap term) : Tac (atom * list atom) =
+  match l with
+  | [] -> fail "Couldn't find return_post term"
+  | hd::tl ->
+      if term_appears_in (`return_post) (select hd am) then hd, tl else
+      let ret, rest = return_at_top tl am in
+      ret, hd::rest
+
+let gather_return (eq: term) (m: term) (lhs rhs:term) : Tac unit =
+  let lhs, rhs =
+    // Ensure that the return_post is on the left
+    if term_appears_in (`return_post) rhs then
+      (apply_lemma (`Steel.Memory.Tactics.equiv_sym); rhs, lhs) else lhs, rhs
+  in
+
+  let m_unit = norm_term [iota; zeta; delta](`CM?.unit (`#m)) in
+  let am = const m_unit in (* empty map *)
+  let (r1_raw, ts, am) = reification eq m [] am lhs in
+  let (r2_raw,  _, am) = reification eq m ts am rhs in
+
+  let l1_raw = flatten r1_raw in
+  let new_l1, emps = return_at_top l1_raw am in
+
+  let am = convert_am am in
+  let r1 = quote_exp r1_raw in
+  let r2 = quote_exp r2_raw in
+
+  change_sq (`(mdenote (`#eq) (`#m) (`#am) (`#r1)
+                 `EQ?.eq (`#eq)`
+               mdenote (`#eq) (`#m) (`#am) (`#r2)));
+
+  apply (`monoid_reflect );
+
+  let l1 = quote_atoms (new_l1 :: emps) in
+  let l2 = quote_atoms (flatten r2_raw) in
+
+  apply_lemma (`equivalent_sorted (`#eq) (`#m) (`#am) (`#l1) (`#l2));
+
+  norm [primops; iota; zeta; delta_only
+    [`%xsdenote; `%select; `%List.Tot.Base.assoc; `%List.Tot.Base.append;
+      `%flatten; `%sort;
+      `%return_post;
+      `%List.Tot.Base.sortWith; `%List.Tot.Base.partition;
+      `%List.Tot.Base.bool_of_compare; `%List.Tot.Base.compare_of_bool;
+      `%fst; `%__proj__Mktuple2__item___1;
+      `%snd; `%__proj__Mktuple2__item___2;
+      `%__proj__CM__item__unit;
+      `%__proj__CM__item__mult;
+      `%Steel.Memory.Tactics.rm
+
+      ]];
+
+  split();
+  split();
+  // equivalent_lists should have built valid permutations.
+  // If that's not the case, it is a bug in equivalent_lists
+  or_else trefl (fun _ -> fail "first equivalent_lists did not build a valid permutation");
+  or_else trefl (fun _ -> fail "second equivalent_lists did not build a valid permutation");
+
+  let n = List.Tot.Base.length emps in
+
+  n_identity_left n eq m
+
+let canon_return' (eq:term) (m:term) : Tac unit =
+  norm [iota; zeta];
+  let t = cur_goal () in
+  // removing top-level squash application
+  let sq, rel_xy = collect_app_ref t in
+  // unpacking the application of the equivalence relation (lhs `EQ?.eq eq` rhs)
+  (match rel_xy with
+   | [(rel_xy,_)] -> (
+       let open FStar.List.Tot.Base in
+       let rel, xy = collect_app_ref rel_xy in
+       if (length xy >= 2)
+       then (
+         match index xy (length xy - 2) , index xy (length xy - 1) with
+         | (lhs, Q_Explicit) , (rhs, Q_Explicit) ->
+           gather_return eq m lhs rhs
+         | _ -> fail "Goal should have been an application of a binary relation to 2 explicit arguments"
+       )
+       else (
+         fail "Goal should have been an application of a binary relation to n implicit and 2 explicit arguments"
+       )
+     )
+   | _ -> fail "Goal should be squash applied to a binary relation")
+
+let canon_return () : Tac unit =
+  canon_return' (`Steel.Memory.Tactics.req) (`Steel.Memory.Tactics.rm)
+
 let rec slterm_nbr_uvars (t:term) : Tac int =
   match inspect t with
   | Tv_Uvar _ _ -> 1
@@ -951,14 +1081,15 @@ let rec solve_subcomp_post (l:list goal) : Tac unit =
 let is_return_eq (l r:term) : Tac bool =
   let nl, al = collect_app l in
   let nr, ar = collect_app r in
-  match al, ar with
-  | [(t1, _)], [(t2, _)] ->
-    let b1 = is_uvar nl in
-    let b2 = is_uvar nr in
-    let b3 = not (is_uvar t1) in
-    let b4 = not (is_uvar t2) in
-    b1 && b2 && b3 && b4
-  | _ -> false
+  term_eq nl (`return_pre) || term_eq nr (`return_pre)
+  // match al, ar with
+  // | [(t1, _)], [(t2, _)] ->
+  //   let b1 = is_uvar nl in
+  //   let b2 = is_uvar nr in
+  //   let b3 = not (is_uvar t1) in
+  //   let b4 = not (is_uvar t2) in
+  //   b1 && b2 && b3 && b4
+  // | _ -> false
 
 let rec solve_indirection_eqs (l:list goal) : Tac unit =
   match l with
@@ -983,6 +1114,36 @@ let rec solve_all_eqs (l:list goal) : Tac unit =
         solve_all_eqs tl
     | _ -> later(); solve_all_eqs tl
 
+// The term corresponds to a goal containing a return_post
+let solve_return (t:term) : Tac unit
+  = // Remove potential annotations first
+    norm [delta_only [`%annot_sub_post; `%delay]];
+    if term_appears_in (`can_be_split) t then (
+      norm [delta_only [`%can_be_split]]
+    ) else if term_appears_in (`can_be_split_forall) t then (
+      ignore (forall_intro ());
+      norm [delta_only [`%can_be_split_forall]]
+    ) else
+      // This should never happen
+      fail "return_post goal in unexpected position";
+    apply_lemma (`equiv_sl_implies);
+    norm [delta_only [
+           `%__proj__CM__item__unit;
+           `%__proj__CM__item__mult;
+           `%Steel.Memory.Tactics.rm;
+           `%__proj__Mktuple2__item___1; `%__proj__Mktuple2__item___2;
+           `%fst; `%snd];
+         primops; iota; zeta];
+    canon_return ()
+
+let rec solve_all_returns (l:list goal) : Tac unit =
+  match l with
+  | [] -> ()
+  | hd::tl ->
+    let t = goal_type hd in
+    let f = term_as_formula' t in
+    if term_appears_in (`return_post) t then solve_return t else later();
+    solve_all_returns tl
 
 let rec solve_triv_eqs (l:list goal) : Tac unit =
   match l with
@@ -1084,7 +1245,11 @@ let init_resolve_tac () : Tac unit =
   // We first need to solve the trivial equalities to ensure we're not restricting
   // scopes for annotated slprops
 //  solve_triv_eqs (goals ());
+  // dump "all initial";
   solve_indirection_eqs (goals());
+  dump "post indirections";
+  solve_all_returns (goals ());
+
   solve_subcomp_pre (goals ());
   // TODO: If we had better handling of lifts from PURE, we might prove a true
   // sl_implies here, "losing" extra assertions"
