ulib/experimental/Steel.Effect.fsti
@@ -59,7 +59,7 @@ let return_ens (a:Type) (x:a) (p:a -> slprop u#1) : ens_t (p x) a p = fun _ r _ 
  * Return is parametric in post (cf. return-scoping.txt)
  *)
 val return (a:Type) (x:a) (#[@@ framing_implicit] p:a -> slprop)
-: repr a (p x) p (return_req (p x)) (return_ens a x p)
+: repr a (return_pre (p x)) (return_post p) (return_req (p x)) (return_ens a x p)
 
 (*
  * We allow weakening of post resource of f to pre resource of g
